traverse.v: abandon the idea of relying on [default m = true]; instead, in [visit], use an explicit bounds check. Prove that [visit] builds a DFS forest. Prove that [visit] satisfies a fixed point equation.

theories/traverse.v
@@ -11,13 +11,14 @@
 (******************************************************************************)
 
 From stdpp Require Import numbers list.
+From stdpp Require Import sets propset.
 From listz Require Import listz.
 Notation len := length.
 From Stdlib Require Import Uint63.
 From Stdlib Require Import Array.PArray.
 From Stdlib Require Export ZifyNat ZifyUint63.
 From marble Require Import tactics bool int iteration loop wp array.
-From marble.logic Require Import olt.
+From marble.logic Require Import relations dfs.
 From marble Require Import listz_buffer. (* TODO *)
 Implicit Type _i _j _k _n : int.
 
@@ -33,12 +34,15 @@ Set Universe Polymorphism.
    This assumption allows us to mark vertices by maintaining an array of
    Boolean marks. This is simple and efficient. *)
 
-Local Notation vertex := int.
+Local Notation _vertex := int.
 Local Notation marks  := (array bool).
 
-Implicit Type v w : vertex.
-Implicit Type vs ws : list vertex.
+Implicit Type _v _w : _vertex.
+Implicit Type _vs _ws : list _vertex.
 Implicit Type m : marks.
+
+Local Notation vertex := Z.
+Implicit Type v w : vertex.
 
 (* -------------------------------------------------------------------------- *)
 
@@ -49,33 +53,8 @@ Implicit Type m : marks.
 Local Definition unmarked (b : bool) : nat :=
   if b then 0 else 1.
 
-(* We wish to record the invariant [default m = true]. That is, outside of
-   the bounds of the marks array, every vertex is considered marked.
-   Therefore, if an out-of-bounds vertex is encountered, then the
-   algorithm ignores it. This lets us prove termination without imposing
-   any conditions on the vertices that the algorithm receives as
-   parameters. Of course, later on (a posteriori), we can use [wp]-style
-   specifications to ensure that every vertex lies within the desired
-   bounds. *)
-
-(* To record this invariant, we use a partial measure. That is, instead
-   of [mweight : marks → nat], we define [mweight : marks → option nat],
-   with the convention that if [m] does not satisfy the invariant then
-   [mweight m] is [None]. *)
-
-(* Because [None] is not an accessible element of the ordering that we
-   impose on the type [option nat], a witness of accessibility of
-   [mweight m] implies that [mweight m] is not [None], therefore implies
-   that [m] satisfies the invariant. *)
-
-Definition mweight m : option nat :=
-  if default m then Some (sum_with unmarked m) else None.
-
-Local Notation olt :=
-  (@olt nat Nat.lt).
-
-Local Notation ole :=
-  (@ole nat Nat.lt).
+Definition mweight m : nat :=
+  sum_with unmarked m.
 
 (* -------------------------------------------------------------------------- *)
 
@@ -101,14 +80,14 @@ Definition weight s :=
 
 (* We write [safe s] for the type of an accessibility witness. *)
 
-Definition safe s :=
-  Acc olt (weight s).
+Notation safe s :=
+  (Acc lt (weight s)).
 
 (* The notations [s' ≤ s] and [s' < s] help reason about the weight
    of a state without visual overhead. *)
 
-Definition slt s' s := olt (weight s') (weight s).
-Definition sle s' s := ole (weight s') (weight s).
+Definition slt s' s := lt (weight s') (weight s).
+Definition sle s' s := le (weight s') (weight s).
 Declare Scope state_scope.
 Infix "≤" := sle (at level 70) : state_scope.
 Infix "<" := slt (at level 70) : state_scope.
@@ -127,7 +106,7 @@ Definition below s :=
 (* [pack_beyond s] wraps the state [s] so that it has type [beyond s]. *)
 
 Definition pack_beyond s : beyond s :=
-  Specif.exist _ s (ole_refl (weight s)).
+  Specif.exist _ s (Nat.le_refl (weight s)).
 
 (* [pack_below s ow] packages the state [s'] and the witness [ow : s' < s]
    so that they have type [beyond s]. *)
@@ -141,8 +120,7 @@ Definition pack_below {s} s' (ow : s' < s) : below s :=
 Local Definition step {s1 s2} : s1 < s2 → beyond s1 → below s2.
 Proof.
   intros ow12 (s0 & ow01). exists s0.
-  unfold sle, slt in *.
-  eauto using ole_olt_trans with typeclass_instances.
+  unfold sle, slt in *. eauto using Nat.le_lt_trans.
 Defined.
 
 (* [decay], an identity function on states, proves that if a state [s']
@@ -151,78 +129,59 @@ Defined.
 Local Definition decay {s} : below s → beyond s.
 Proof.
   intros (s' & ow). exists s'.
-  unfold slt, sle in *.
-  eauto using olt_ole with typeclass_instances.
+  unfold slt, sle in *. eauto using Nat.lt_le_incl.
 Defined.
 
-(* [decrease] constructs a strict ordering witness, expressing the idea
-   that if the vertex [v] is unmarked in the state [s], which is the pair
-   [(m, u)], then marking [v] produces a new state of smaller weight. *)
+(* [step] and [decay] are identity functions, so, while reasoning via
+   [wpd] judgements, they have no effect. *)
 
-Lemma decrease s m v u u' :
+Local Lemma wpd_step {s1 s2} (a : beyond s1) (pf : s1 < s2) Q :
+  wpd a Q →
+  wpd (step pf a) Q.
+Proof.
+  unfold step. destruct a. tauto.
+Qed.
+
+Local Lemma wpd_decay {s} (a : below s) Q :
+  wpd a Q →
+  wpd (decay a) Q.
+Proof.
+  unfold decay. destruct a. tauto.
+Qed.
+
+(* [decrease] constructs a strict ordering witness, expressing the idea
+   that if the vertex [_v] is unmarked in the state [s], which is the pair
+   [(m, u)], then marking [_v] produces a new state of smaller weight. *)
+
+Lemma decrease s m _v u u' :
   s = (m, u) →
   safe s →
-  get m v = false →
-  (set m v true, u') < s.
+  (_v <? length m)%uint63 = true →
+  get m _v = false →
+  (set m _v true, u') < s.
 Proof.
-  intros ? Hsafe Hget. subst.
-  (* The beautiful hack: from [safe (m, u)],
-     we deduce [default m = true]. *)
-  assert (Hm: default m = true).
-  { unfold safe, weight, mweight in *.
-    (* By way of contradiction, assume [default m] is [false]. *)
-    destruct (default m) eqn:Hm; [ reflexivity | exfalso ].
-    (* Then we get that [None] is accessible. Contradiction. *)
-    eapply (@Acc_None nat Nat.lt). tauto. }
-  (* Because [default m] is [true], and because this remains true
-     after [m] is updated, the goal can be simplified and becomes
-     a comparison of two natural numbers. *)
+  intros ? Hsafe Hv Hget. subst.
   unfold slt, weight, mweight.
-  rewrite default_set.
-  rewrite Hm.
-  simpl.
-  (* Furthermore, because [default m] is [true] and [get m v] is [false],
-     the vertex [v] must lie within the bounds of the array [m]. *)
-  assert ((v <? length m)%uint63 = true).
-  { destruct ((v <? length m)%uint63) eqn:Hv; [ reflexivity | exfalso ].
-    apply get_out_of_bounds in Hv.
-    congruence. }
-  (* There remains to work. This is a bit ugly. *)
-  set (i := (φ v)%uint63).
-  assert (unsigned i). { unfold i. lia. }
-  assert (isInt v i).  { eapply introIsInt. reflexivity. }
-  assert (Hvalid: valid i (to_list m))
+  (* This is a bit ugly. *)
+  set (v := (φ _v)%uint63).
+  assert (unsigned v). { unfold v. lia. }
+  assert (isInt _v v).  { eapply introIsInt. reflexivity. }
+  assert (Hvalid: valid v (to_list m))
     by eauto using ltb_length_spec with typeclass_instances.
   rewrite !sum_with_spec.
   erewrite set_spec by eauto.
-  generalize (sum_list_with_insert unmarked i (to_list m) true Hvalid).
+  generalize (sum_list_with_insert unmarked v (to_list m) true Hvalid).
   erewrite <- get_spec by eauto.
   rewrite Hget.
   simpl unmarked.
   lia. (* ouf *)
 Qed.
 
-(* A marks array [m] of arbitrary size [_n], allocated via [init] and
-   initialized with [false] everywhere, is a safe initial state. *)
+(* Every state is safe. *)
 
-(* Fortunately, [n ≤ max_array_length] is not required. *)
-
-Local Lemma safe_init _n u :
-  safe (init _n (λ _, false), u).
+Local Lemma all_safe s : safe s.
 Proof.
-  (* We rely on the fact that [inhabitant] at type [bool] happens to
-     be [true]. We need the array [m] to be everywhere [false] and to
-     have default value [true]. *)
-  assert (fact: default (init _n (λ _, false)) = true).
-  { change true with (inhabitant : bool). eapply default_init. }
-  revert fact.
-  generalize (init _n (λ _, false)); intro m.
-  intro Hm.
-  unfold safe, weight, mweight.
-  rewrite Hm; clear Hm.
-  eapply Acc_Some.
-  eapply (Acc_intro_generator 32).
-  eapply Wf_nat.lt_wf.
+  eapply (Acc_intro_generator 32). eapply Wf_nat.lt_wf.
 Defined.
 
 (* -------------------------------------------------------------------------- *)
@@ -231,27 +190,23 @@ Defined.
 
 Section Visit.
 
-(* [foreach_successor v] must iterate on the successors of the vertex [v]. *)
+(* [foreach_successor a _v] iterates on the successors of the vertex [_v]. *)
 
 (* Fortunately, no properties of this function are needed in the proof of
    termination of [visit]. *)
 
-Variable foreach_successor : ∀ {A}, A → vertex → (A → vertex → A) → A.
+Variable foreach_successor : ∀ {A}, A → _vertex → (A → _vertex → A) → A.
 
-(* The user function [body v u] is invoked when a vertex [v] is discovered.
-   It updates the user state [u]. *)
+(* The user function [body _v u] is invoked when a vertex [_v] is
+   discovered. It updates the user state [u]. *)
 
-Variable body : vertex → U → U.
+Variable body : _vertex → U → U.
 
-(* [visit] expects a state [s], a vertex [v], and a proof that this state
-   is safe. The fact that [s] is safe (accessible) is used to justify
-   termination; the function is defined by structural recursion on [ACC]. *)
+(* [visit] expects a state [s], a vertex [_v], and a proof that [s] is
+   safe (accessible). This proof is used to justify termination; the
+   function is defined by structural recursion on [ACC]. *)
 
-(* Thanks to the beautiful hack, there is no need to separately keep track
-   of an invariant about the state [s]. A state that does not satisfy the
-   invariant is deemed inaccessible (unsafe). *)
-
-(* [visit s v ACC] produces a result of type [beyond s], that is, a new
+(* [visit s _v ACC] produces a result of type [beyond s], that is, a new
    state [s'] such that [s' ≤ s] holds. This information is required,
    while iterating on the successors of a state, to prove that every call
    to [visit] in this sequence is permitted. *)
@@ -262,23 +217,24 @@ Variable body : vertex → U → U.
    require an accessibility witness as an argument. Fortunately, this is
    possible! *)
 
-Fixpoint visit s v (ACC : safe s) : beyond s :=
-  (* Destruct [s] as a pair [(m, u)] while keeping track of the equation. *)
+Fixpoint visit s _v (ACC : safe s) : beyond s :=
+  (* Destruct [s] as a pair [m, u] while keeping track of the equation. *)
   match s as b return s = b → _ with (m, u) => λ Hsmu,
-  (* Test whether the vertex [v] is marked. *)
-  let marked := get m v in
-  IFC marked THEN λ _,
+  (* Test whether this vertex is valid. *)
+  IFC (_v <? length m)%uint63 THEN λ Hv,
+  (* Test whether this vertex is marked. *)
+  IFC get m _v THEN λ _,
     (* It is marked: do nothing. *)
     pack_beyond s
   ELSE λ Hunmarked,
     (* Mark this vertex. *)
-    let m' := set m v true in
+    let m' := set m _v true in
     (* Invoke the user function [body]. *)
-    do u' ← body v u ;
+    do u' ← body _v u ;
     (* Construct an updated state. *)
     let s' := (m', u') in
     (* Construct a witness of the assertion [s' < s]. *)
-    let ow : s' < s := decrease s m v u u' Hsmu ACC Hunmarked in
+    let ow : s' < s := decrease s m _v u u' Hsmu ACC Hv Hunmarked in
     (* Package them together. *)
     let s' := pack_below s' ow in
     (* Package [visit] as a function of type [below s → vertex → below s],
@@ -287,14 +243,335 @@ Fixpoint visit s v (ACC : safe s) : beyond s :=
        Therefore we are able to package [visit] as a function that does
        not require an accessibility witness. *)
     (* This construction has just [visit] and [ACC] as free variables. *)
-    let visit (sow' : below s) (w : vertex) : below s :=
+    let visit (sow' : below s) (_w : _vertex) : below s :=
       let (s', ow) := sow' in
-      step ow (visit s' w (Acc_inv ACC ow))
+      step ow (visit s' _w (Acc_inv ACC ow))
     in
     (* Visit the successors of [v], *)
     (* Visit them, then use [decay] to forget that we went below [s]. *)
-    decay (foreach_successor s' v visit)
+    decay (foreach_successor s' _v visit)
+  ELSE λ _,
+     (* This vertex is out-of-bounds. Ignore it. This lets us prove
+        termination without imposing any conditions on the vertices
+        that we receive. *)
+    pack_beyond s
   end eq_refl.
+
+(* In an earlier version of this code, we did not test whether [v] is
+   valid. Instead, we relied on the hypothesis [default m = true], which
+   implies that if [v] is out-of-bounds then it is considered marked
+   already. This would force us to establish and keep track of the
+   invariant [default m = true]. It was a bit cumbersome and inelegant,
+   as we usually never access the default element of an array and never
+   need to keep track of its value. Furthermore, this approach led us to
+   a situation where Rocq's type-checker would not terminate. Therefore
+   we have abandoned it. *)
+
+(* -------------------------------------------------------------------------- *)
+
+(* We now formulate more hypotheses about the functions [foreach_successor]
+   and [body], which the user provides. Under these hypotheses, we prove
+   that [visit] is correct. *)
+
+(* The vertices must form a directed graph. *)
+
+Variable E : relation vertex.
+
+(* The vertices must be numbered from 0 to [n], excluded. *)
+
+Variable n : Z.
+
+(* No edge can leave the interval [0, n). *)
+
+Hypothesis bound :
+  ∀ v w, 0 ≤ v < n → E v w → 0 ≤ w < n.
+
+(* The function [foreach_successor], applied to [_v], must enumerate the
+   successors of the vertex [v]. They can be enumerated in an arbitrary
+   order, and it is permitted for a vertex [w] to be presented several
+   times. *)
+
+Local Notation successors v :=
+  (image E {[v]}).
+
+Variable wp_foreach_successor:
+  ∀ {A} (body : A → _vertex → A),
+  ∀Int _v v,
+  0 ≤ v < n →
+  ITER_SET ∅ (successors v)
+    (λ w a Q, ∀ _w, isInt _w w → wp (body a _w) Q)
+    (λ a Q, wp (foreach_successor a _v body) Q).
+
+(* The function [body], applied to a vertex [_v] and to a user state [u],
+   returns a new user state. *)
+
+(* TODO add a user invariant on [u] *)
+
+Variable wp_body :
+  ∀Int _v v,
+  0 ≤ v < n →
+  ∀ u,
+  wp (body _v u) (λ u, True).
+
+(* -------------------------------------------------------------------------- *)
+
+(* [marked], [imarked], [omarked] denote sets of vertices. *)
+
+Local Notation vertices := (propset vertex).
+Implicit Types marked imarked omarked : vertices.
+
+(* [isMarks m marked] means that the Boolean array [m] represents the set
+   of vertices [marked]. *)
+
+Open Scope Z_scope.
+
+Definition isMarks m marked :=
+  ∃ bs,
+  isArray m bs ∧
+  len bs = n ∧
+  ∀ v, 0 ≤ v < n → isBool1 (bs !!! v) (v ∈ marked).
+
+Local Ltac introMarks :=
+  eexists; split; [| split]; [ isArray | list; tc | ].
+
+Local Ltac destructMarks :=
+  match goal with h: isMarks _ _ |- _ =>
+    generalize h; intro; (* keep a copy *)
+    let bs := fresh "bs" in
+    destruct h as (bs & ? & ? & ?)
+  end.
+
+Local Instance isBool_get_mark m marked :
+  ∀Int _v v,
+  0 ≤ v < n →
+  isMarks m marked →
+  isBool1 (get m _v) (v ∈ marked).
+Proof.
+  intros. destructMarks.
+  assert (fact: wp (get m _v) (eq (bs !!! v))).
+  { wp_get b. eauto. }
+  rewrite wp_iff in fact.
+  rewrite <- fact. tc.
+Qed.
+
+Local Lemma mark_self marked v : v ∈ {[v]} ∪ marked.
+Proof. set_solver. Qed.
+Local Hint Resolve mark_self : marble.
+
+Local Lemma mark_unaffected marked v v' :
+  v ≠ v' →
+  v' ∈ {[v]} ∪ marked ↔ v' ∈ marked.
+Proof. set_solver. Qed.
+
+(* -------------------------------------------------------------------------- *)
+
+(* The assertion [dfs imarked omarked f], defined in dfs.v, means that [f]
+   is a DFS forest for the graph [E], consistent with the set of initially
+   marked vertices [imarked] and with the set of finally marked vertices
+   [omarked]. *)
+
+Implicit Type f : forest vertex.
+
+Local Notation dfs := (@dfs vertex E).
+
+(* The postcondition of [visit]. *)
+
+(* [visit_post imarked examined s'] means that, if one starts from the set
+   of initially marked vertices [imarked] and if the roots of the search
+   form the set [examined], then [s'] is a correct final state. *)
+
+Definition visit_post imarked examined s' :=
+  let (m', u') := s' in
+  ∃ omarked f,
+  isMarks m' omarked ∧
+  examined ⊆ omarked ∧
+  dfs imarked omarked f ∧
+  roots f ⊆ examined.
+
+Local Ltac intro_visit_post :=
+  unfold visit_post; do 2 eexists; pack;
+    [ eauto | set_solver | |].
+
+Local Ltac intro_visit_post_empty :=
+  intro_visit_post; [ eapply DFSEmpty; eauto | set_solver ].
+
+Local Ltac elim_visit_post omarked f :=
+  match goal with h: visit_post _ _ _ |- _ =>
+    unfold visit_post in h;
+    destruct h as (omarked & f & ? & ? & ? & ?);
+    dfs_monotonic
+  end.
+
+(* The specification of [visit]. *)
+
+(* Because the result type of [visit] is a subset type,
+   instead of [wp], we use the judgement [wpd]. *)
+
+Lemma wpd_visit (k : nat) :
+  ∀ m u _v v ACC imarked,
+  mweight m = k →
+  isMarks m imarked →
+  isInt _v v →
+  0 ≤ v < n →
+  wpd (visit (m, u) _v ACC) (λ s', visit_post imarked {[v]} s').
+Proof.
+  by well-founded induction on k along lt.
+  intros. subst k. destruct ACC. simpl visit.
+  destructMarks. arrays.
+  (* Because we require [v < n], the first branch of this conditional
+     construct must be taken. The second branch is dead. *)
+  eapply wpd_IFC; [ tc | intros | lia ].
+  (* The second conditional construct tests whether [v] is marked. *)
+  eapply wpd_IFC; [ tc | intros | intros ].
+  (* Case: [v] is marked already. *)
+  { eapply wpd_ret. intro_visit_post_empty. }
+  (* Case: [v] is unmarked. We mark this vertex. *)
+  assert (fact: wp (set m _v true) (λ m, isMarks m ({[v]} ∪ imarked))).
+  { wp_set. introMarks. intros v' ?. case_lookup_insert.
+    + subst v'. tc.
+    + rewrite mark_unaffected by assumption. tc. }
+  rewrite wp_iff in fact.
+  revert fact. set (m' := set m _v true).
+  set (marked' := {[v]} ∪ imarked). intro.
+  (* We invoke the user function [body]. *)
+  eapply wpd_bind; last wp_intro u'.
+  { eauto using wp_body. }
+  (* The state at this point is described by [marked'] and [u']. *)
+  eapply wpd_decay.
+  (* We reach the loop on the successors of [v]. The goal must be changed
+     from [wpd] to [wp], so that [wp_foreach_successor] can be used. *)
+  rewrite wpd_wp.
+  wp_op wp_foreach_successor with invariant: (
+    λ examined (s'' : { s'' | slt s'' (m, u) }),
+      visit_post marked' examined (proj1_sig s'')
+  ).
+  (* Initialization. *)
+  { intro_visit_post_empty. }
+  (* Preservation. *)
+  { wp_body examined0 examined1 ((m'' & u'') & ow)
+      introducing: (fun _ => set_step w; intros _w ?).
+    elim_visit_post marked'' f.
+    assert (E v w) by set_solver.
+    (* The state at this point is described by [marked''] and [u''].
+       The successors of [v] that have been examined already form
+       the set [examined0], a subset of [marked'']. The vertex [w],
+       also a successor of [v], is about to be examined. *)
+    (* Change the goal back into [wpd] format. *)
+    eapply wp_wpd with (Q1 := λ s'', visit_post marked' examined1 s'');
+      [| solve [ eauto] ].
+    eapply wpd_step.
+    (* Use the induction hypothesis to justify calling [visit s'' _w ]. *)
+    eapply wpd_conseq.
+    { eapply IH; try reflexivity; tc. }
+    (* Justify that this call establishes the loop invariant. *)
+    cbv beta. intros (m''' & u''') ?.
+    elim_visit_post omarked f'''.
+    intro_visit_post.
+    + eauto using dfs_concat.
+    + rewrite roots_concat. set_solver. }
+  (* Completion. All successors of [v] have now been examined. *)
+  { intros ((m'' & u'') & ?). simpl proj1_sig.
+    intros (examined & ? & ?).
+    elim_visit_post omarked f.
+    intro_visit_post.
+    + eapply DFSNonEmpty with (w := v); eauto with dfs set_solver.
+    + set_solver. }
+Qed.
+
+(* -------------------------------------------------------------------------- *)
+
+(* Once the termination of [visit] has been established, one can define a
+   simplified version of it, which does not need an accessibility witness,
+   and whose result type is just [S]. *)
+
+Definition visit' s _v : S :=
+  proj1_sig (visit s _v (all_safe s)).
+
+(* As an exercise, we prove that [visit'] satisfies the desired fixed
+   point equation. Most likely, we will NOT need this property. I am
+   showing this proof for pedagogical purposes; it is super difficult
+   if one does not approach it in exactly the right way. *)
+
+(* Under [proj1_sig], the coercions [step] and [decay] vanish. *)
+
+Lemma proj1_sig_step {s1 s2} (pf : slt s1 s2) (s' : beyond s1) :
+  proj1_sig (step pf s') = proj1_sig s'.
+Proof.
+  destruct s'. eauto.
+Qed.
+
+Lemma proj1_sig_decay {s} (s' : below s) :
+  proj1_sig (decay s') = proj1_sig s'.
+Proof.
+  destruct s'. eauto.
+Qed.
+
+(* Because [foreach_successor] is an unknown function, we must assume
+   that it is parametric: that is, when applied to related arguments,
+   it produces related results. *)
+
+Hypothesis foreach_successor_parametric:
+  ∀ {A1 A2} (A : A1 → A2 → Prop),
+  ∀ (body1 : A1 → _vertex → A1) (body2 : A2 → _vertex → A2),
+  ( ∀ a1 a2, A a1 a2 →
+    ∀ _w,
+    A (body1 a1 _w) (body2 a2 _w)
+  ) →
+  ∀ a1 a2, A a1 a2 →
+  ∀ _v,
+  A (foreach_successor a1 _v body1) (foreach_successor a2 _v body2).
+
+(* [visit] satisfies the desired fixed point equation: *)
+
+Lemma visit_eq (k : nat) :
+  ∀ s _v ACC,
+  weight s = k →
+  proj1_sig (visit s _v ACC) =
+    let (m, u) := s in
+    if (_v <? length m)%uint63 then
+      do b ← get m _v ;
+      if b then
+        s
+      else
+        do m' ← set m _v true ;
+        do u' ← body _v u ;
+        let s' := (m', u') in
+        foreach_successor s' _v visit'
+    else
+      s.
+Proof.
+  by well-founded induction on k along lt.
+  intros. subst k. destruct ACC as (ACC). simpl visit.
+  destruct s as (m & u).
+  eapply IFC_if_dep; intro; [| eauto ].
+  eapply IFC_if_dep; intro; [ eauto |].
+  unfold bind at 2.
+  eapply bind_eq_dep; [ eauto | intro u' ].
+  rewrite proj1_sig_decay.
+  eapply foreach_successor_parametric
+    with (A := λ (s1 : below (m, u)) (s2 : S), proj1_sig s1 = s2);
+    [| eauto ].
+  intros (s' & ?) ?. simpl. intros <- _w.
+  rewrite proj1_sig_step.
+  unfold visit'.
+  (* The goal boils down to proving that the parameter [ACC] is
+     computationally irrelevant; that is, it does not influence
+     the first projection of the result of [visit]. *)
+  erewrite !IH by eauto. (* rewrite both sides *)
+  reflexivity.
+Qed.
+
+(* -------------------------------------------------------------------------- *)
+
+(* The top-level function does not need an accessibility witness.
+   It allocates the marks array [m]. *)
+
+(* TODO use [foreach_root] *)
+
+Definition visit_top _n u _v : S :=
+  let m := init _n (λ _i, false) in
+  let s := (m, u) in
+  visit' s _v.
 
 End Visit.
 
